src/Formalisation/Formats/Ipsec/esp.v
@@ -1,0 +1,40 @@
+From Formalisation Require Import Span SizeNat.
+From Formalisation Require Import ikev2 Nom combinator bin_combinators ikev2_parser.
+
+Record ESPHeaderS (S :Type) :=
+  mk_espheader {
+      spi_index : S;
+      seq : nat32;
+      data : S
+    }.
+
+Definition ESPHeader := ESPHeaderS span.
+
+Arguments mk_espheader [_].
+Arguments spi_index [_].
+Arguments seq [_].
+Arguments data [_].
+
+Global Instance FOldable_ESPHeader : Foldable ESPHeaderS.
+econstructor.
+intros M sg m A f v. eapply Monoid.f. eapply (f (spi_index v)).
+eapply (f (data v)).
+Defined.
+
+Inductive ESPData :=
+| ESP (e : ESPHeader)
+| IKE (i : IkeV2Header).
+
+Definition parse_esp_header : NomG ESPHeader :=
+  let! spi_index := take 4 in
+  let! seq := be_u32 in
+  let! data := rest in
+  ret (mk_espheader spi_index seq data).
+
+Definition parse_esp_encapsulated : NomG ESPData :=
+  let! v := be_u32 in
+  if val v =? 0
+  then
+    map parse_ikev2_header IKE
+  else
+    map parse_esp_header ESP.
