src/Formalisation/Formats/Ipsec/ikev2_notify.v
@@ -1,8 +1,7 @@
-From Formalisation Require Import Nom SizeNat ikev2_transforms.
+From Formalisation Require Import SizeNat Nom.
 
-Record NotifyType :=
-  mk_notify {
-      val_noti : nat16;
-      is_error : bool := val val_noti <? 16384;
-      is_status : bool := 16384 <? val val_noti
-    }.
+Definition NotifyType := nat16.
+
+Definition is_error (n : NotifyType): bool := val n <? 16384.
+
+Definition is_status (n : NotifyType) : bool := 16384 <? val n.
